examples/seplogic/Lang.fst
@@ -76,7 +76,7 @@ let lemma_join_emp (h1:heap) (h2:heap)
    
 (* let points_to (id:addr) (n:nat) (h:heap) :Type0 = dom h == Set.singleton id /\ h.[id] == n *)
 let points_to (id:addr) (n:nat) (h:heap) : Type0 =
-  (equal h (restrict h (Set.singleton (addr_of id)))) /\ (sel h id == n)
+  (h == (restrict h (Set.singleton (addr_of id)))) /\ (sel h id == n)
 
 let lift (phi:Type0) (h:heap) :Type0 = phi /\ is_emp h
 
@@ -84,7 +84,7 @@ let exists_x (#a:Type0) (pred:a -> heap_predicate) (h:heap) :Type0
   = exists (x:a). pred x h
 
 let star (p:heap_predicate) (q:heap_predicate) (h:heap) :Type0
-  = exists (h1:heap) (h2:heap). disjoint h1 h2 /\ h == join h1 h2 /\ p h1 /\ q h2
+  = exists (h1:heap) (h2:heap). disjoint h1 h2 /\ (h == (join h1 h2)) /\ p h1 /\ q h2
 
 let iff (p:heap_predicate) (q:heap_predicate) :Type0 = forall (h:heap). p h <==> q h
 
@@ -95,28 +95,67 @@ let lemma1_helper (phi:Type0) (p:heap_predicate) (q:heap_predicate) (h:heap)
   :Lemma (requires ((phi ==> (p `imp` q)) /\
                     (star p (lift phi) h)))
          (ensures  (q h))
- = assert (exists (h1:heap) (h2:heap). disjoint h1 h2 /\ (equal h (join h1 h2)) /\ p h1 /\ ((lift phi) h2) /\ is_emp h2 /\ phi /\ q h1)
-
+ = assert (exists (h1:heap) (h2:heap). disjoint h1 h2 /\ (h == (join h1 h2)) /\ p h1 /\ ((lift phi) h2) /\ is_emp h2 /\ phi /\ q h1 /\ (h1 == h))
+ 
 let lemma1 (phi:Type0) (p:heap_predicate) (q:heap_predicate)
   :Lemma (requires (phi ==> (p `imp` q)))
          (ensures ((star p (lift phi)) `imp` q))
   = Classical.forall_intro (Classical.move_requires (lemma1_helper phi p q))
+
 
 let lemma2 (phi:Type0) (p:heap_predicate) (q:heap_predicate)
   :Lemma (requires (phi /\ (p `imp` q)))
          (ensures (p `imp` (star q (lift phi))))
   = assert (forall (h:heap). (p h ==> q h) /\ phi /\ ((lift phi) emp) /\ (disjoint h emp))
 
+
 let lemma3 (phi:Type0) (p:heap_predicate)
   :Lemma (requires phi)
          (ensures (p `iff` (star p (lift phi)))) 
-  = assert (forall (h:heap). phi /\ ((lift phi) emp) /\ (disjoint h emp) /\ (equal h (join h emp)))
+  = assert (forall (h:heap). phi /\ ((lift phi) emp) /\ (disjoint h emp) /\ (h == (join h emp)))
 
-let lemma_star_is_comm (p:heap_predicate) (q:heap_predicate) 
+let lemma4 (p:heap_predicate) (q:heap_predicate) 
   :Lemma (requires True)
          (ensures (star p q) `iff` (star q p))
   = assert (forall (h1:heap) (h2:heap). (disjoint h1 h2) <==> (disjoint h2 h1))
+
+(*
+let lemma5_helper (p:heap_predicate) (q:heap_predicate) (r:heap_predicate) (h:heap)
+  :Lemma (requires (star p (star q r) h))
+         (ensures (star (star p q) r h))
+  = assert (exists (h1:heap) (h2:heap) (h3:heap). p h1 /\ q h2 /\ r h3 /\ disjoint h2 h3 /\ (disjoint h1 (join h2 h3)) /\ (h == (join h1 (join h2 h3))) /\ (disjoint h1 h3) /\ (disjoint h3 h1 /\ disjoint h3 h2) /\ disjoint h3 (join h1 h2) /\ (h == (join h3 (join h1 h2))))
+
+*)
+
+let lemma5 (p:heap_predicate) (q:heap_predicate) (r:heap_predicate)
+  :Lemma (requires True)
+         (ensures (star p (star q r)) `iff` (star (star p q) r))
+  = ()
   
+  
+(*   assert (exists (h1:heap) (h2:heap) (h3:heap). p h1 /\ q h2 /\ r h3 /\ (disjoint h2 h3) /\ (disjoint h1 (join h2 h3)))
+*)
+
+let lemma6 (p1:heap_predicate) (p2:heap_predicate) (q1:heap_predicate) (q2:heap_predicate)
+  :Lemma (requires ((p1 `imp` p2) /\ (q1 `imp` q2)))
+         (ensures ((star p1 q1) `imp` (star p2 q2)))
+  = ()
+
+let lemma7 (#a:Type0) (p:heap_predicate) (q:a -> heap_predicate)
+  :Lemma (requires True)
+         (ensures (star p (exists_x (fun x -> (q x)))) `iff` (exists_x (fun x -> star p (q x))))
+  = ()
+
+let lemma8 (#a:Type0) (p:a -> heap_predicate) (q:heap_predicate)
+  :Lemma (requires (forall (x:a). (p x) `imp` q))
+         (ensures (exists_x p) `imp` q)
+  = ()
+  
+let lemma9 (#a:Type0) (p:heap_predicate) (q:a -> heap_predicate) (v:a)
+  :Lemma (requires (p `imp` (q v)))
+         (ensures (p `imp` exists_x (q)))
+  = ()
+
 type c_pre            = heap_predicate
 type c_post (a:Type0) = a -> heap_predicate
 
@@ -179,7 +218,10 @@ let lemma_free (id:addr)
 				 (fun _ -> is_emp)))
   = admit ()
 
+let lemma_frame_rule (#a:Type0) (c:command a) (p:c_pre) (q:c_post a) (r:c_pre)
+  :Lemma (requires hoare_triple p c q)
+         (ensures hoare_triple (p `star` r) c (fun x -> (q x) `star` r))
+  = admit ()
+          
 (* get the nice x <-- c1; c2 syntax *)
 let bind (#a:Type0) (#b:Type0) (c1:command a) (c2:a -> command b) :command b = Bind c1 c2
-
-
